

Double Pendulum EOMs

Locations of pendulum bobs:

$$\begin{cases} x_1 = l_1 \sin \alpha_1 \\ x_2 = l_1 \sin \alpha_1 + l_2 \sin \alpha_2 \\ y_1 = -l_1 \cos \alpha_1 \\ y_2 = -l_1 \cos \alpha_1 - l_2 \cos \alpha_2 \end{cases} \quad (1)$$

Lagrangian of pendulum bob positions:

$$\begin{cases} T = \frac{m_1 v_1^2}{2} + \frac{m_2 v_2^2}{2} = \frac{m_1(\dot{x}_1^2 + \dot{y}_1^2)}{2} + \frac{m_2(\dot{x}_2^2 + \dot{y}_2^2)}{2} \\ V = m_1 g y_1 + m_2 g y_2 \end{cases} \quad (2)$$

$$L = T - V = \frac{m_1(\dot{x}_1^2 + \dot{y}_1^2)}{2} + \frac{m_2(\dot{x}_2^2 + \dot{y}_2^2)}{2} - m_1 g y_1 - m_2 g y_2 \quad (3)$$

Lagrangian in generalized coordinates:

$$\begin{cases} \dot{x}_1^2 = l_1^2 \dot{\alpha}_1^2 \cos^2 \alpha_1 \\ \dot{x}_2^2 = l_1^2 \dot{\alpha}_1^2 \cos^2 \alpha_1 + l_2^2 \dot{\alpha}_2^2 \cos^2 \alpha_2 + 2 l_1 l_2 \dot{\alpha}_1 \dot{\alpha}_2 \cos \alpha_1 \cos \alpha_2 \\ \dot{y}_1^2 = l_1^2 \dot{\alpha}_1^2 \sin^2 \alpha_1 \\ \dot{y}_2^2 = l_1^2 \dot{\alpha}_1^2 \sin^2 \alpha_1 + l_2^2 \dot{\alpha}_2^2 \sin^2 \alpha_2 + 2 l_1 l_2 \dot{\alpha}_1 \dot{\alpha}_2 \sin \alpha_1 \sin \alpha_2 \end{cases} \quad (4)$$

$$\begin{aligned} L = T - V = & \frac{(m_1 + m_2) l_1^2 \dot{\alpha}_1^2 + m_2 l_2^2 \dot{\alpha}_2^2}{2} \\ & + m_2 l_1 l_2 \dot{\alpha}_1 \dot{\alpha}_2 \cos(\alpha_1 - \alpha_2) \\ & + (m_1 + m_2) g l_1 \cos \alpha_1 \\ & + m_2 g l_2 \cos \alpha_2 \end{aligned} \quad (5)$$

Lagrangian equations of motion

$$\frac{d}{dt} \frac{\partial L}{\partial \dot{\alpha}_i} - \frac{\partial L}{\partial \alpha_i} = 0, \quad i = 1, 2 \quad (6)$$

$$\left\{ \begin{array}{l} \frac{\partial L}{\partial \dot{\alpha}_1} = (m_1 + m_2)l_1^2 \dot{\alpha}_1 + m_2 l_1 l_2 \dot{\alpha}_2 \cos(\alpha_1 - \alpha_2) \\ \frac{\partial L}{\partial \alpha_1} = -m_2 l_1 l_2 \dot{\alpha}_1 \dot{\alpha}_2 \sin(\alpha_1 - \alpha_2) - (m_1 + m_2)g l_1 \sin \alpha_1 \\ \frac{\partial L}{\partial \dot{\alpha}_2} = m_2 l_2^2 \dot{\alpha}_2 + m_2 l_1 l_2 \dot{\alpha}_1 \cos(\alpha_1 - \alpha_2) \\ \frac{\partial L}{\partial \alpha_2} = m_2 l_1 l_2 \dot{\alpha}_1 \dot{\alpha}_2 \sin(\alpha_1 - \alpha_2) - m_2 g l_2 \sin \alpha_2 \end{array} \right. \quad (7)$$

From (6) and (7), we can get the 2 equations of motion for double pendulum:

$$\left\{ \begin{array}{l} (m_1 + m_2)l_1 \ddot{\alpha}_1 + m_2 l_2 \ddot{\alpha}_2 \cos(\alpha_1 - \alpha_2) + m_2 l_2 \dot{\alpha}_2^2 \sin(\alpha_1 - \alpha_2) + (m_1 + m_2)g \sin \alpha_1 = 0 \\ l_2 \ddot{\alpha}_2 + l_1 \ddot{\alpha}_1 \cos(\alpha_1 - \alpha_2) - l_1 \dot{\alpha}_1^2 \sin(\alpha_1 - \alpha_2) + g \sin \alpha_2 = 0 \end{array} \right. \quad (8)$$

Substitute equations into each other, we get:

$$\left\{ \begin{array}{l} \ddot{\alpha}_1 = \frac{A}{m_1 l_1 + m_2 l_1 \sin^2(\alpha_1 - \alpha_2)}, \quad \text{where} \\ A = -m_2 l_1 \sin(\alpha_1 - \alpha_2) \cos(\alpha_1 - \alpha_2) \dot{\alpha}_1^2 + m_2 g \cos(\alpha_1 - \alpha_2) \sin \alpha_2 \\ \quad - m_2 l_2 \dot{\alpha}_2^2 \sin(\alpha_1 - \alpha_2) - (m_1 + m_2)g \sin \alpha_1 \\ \ddot{\alpha}_2 = \frac{B}{m_1 l_2 + m_2 l_2 \sin^2(\alpha_1 - \alpha_2)}, \quad \text{where} \\ B = (m_1 l_1 + m_2 l_1) \dot{\alpha}_1^2 \sin(\alpha_1 - \alpha_2) + m_2 l_2 \dot{\alpha}_2 \sin(\alpha_1 - \alpha_2) \cos(\alpha_1 - \alpha_2) \\ \quad + (m_1 + m_2)g \sin \alpha_1 \cos(\alpha_1 - \alpha_2) - (m_1 + m_2)g \sin \alpha_2 \end{array} \right. \quad (9)$$